Vector_of_tuple.v
@@ -1,0 +1,66 @@
+(* This file is originated from
+  https://gist.github.com/qnighy/bad737efac4b1bc9b9fc *)
+
+Require Import ssreflect ssrfun ssrbool eqtype ssrnat seq fintype.
+Require Import tuple finfun finset.
+Require Import Coq.Vectors.Vector.
+
+Lemma beheadE n T (x : T) (t : n.-tuple T) :
+    behead_tuple [tuple of x :: t] = t.
+Proof.
+  by apply val_inj.
+Qed.
+
+Section tuple_Vector_correspondence.
+  Variable T : Type.
+
+  Fixpoint tuple_of_Vector(n:nat) :=
+    match n return Vector.t T n -> tuple_of n T with
+    | 0 => fun _ => [tuple]
+    | n'.+1 => fun v =>
+        [tuple of Vector.hd v :: tuple_of_Vector n' (Vector.tl v)]
+    end.
+
+  Fixpoint Vector_of_tuple(n:nat) :=
+    match n return tuple_of n T -> Vector.t T n with
+    | 0 => fun _ => Vector.nil T
+    | n'.+1 => fun t =>
+        Vector.cons T (thead t) n' (Vector_of_tuple n' (behead_tuple t))
+    end.
+
+  Lemma tuple_of_VectorK n :
+      cancel (@tuple_of_Vector n) (@Vector_of_tuple n).
+  Proof.
+    elim: n; first by move=> /=; apply case0.
+    move=> n /= H v.
+    move: n v H.
+    refine (@caseS T _ _).
+    move => vh n vt H /=.
+    congr 2 (fun vh => cons T vh n).
+    by rewrite beheadE H.
+  Qed.
+
+  Lemma VectorK_of_tuple n :
+      cancel (@Vector_of_tuple n) (@tuple_of_Vector n).
+  Proof.
+    elim: n; first by move=> x; symmetry; apply tuple0.
+    move=> n /= H t.
+    by rewrite H -tuple_eta.
+  Qed.
+End tuple_Vector_correspondence.
+
+
+(* Explanation of a problem *)
+
+Parameter Sg : nat -> eqType.
+
+Fail Inductive Term :=
+  | Tvar : nat -> Term
+  | Tope n : Sg n -> n.-tuple Term -> Term.
+(* Error: Non strictly positive occurrence of "Term" in
+    "forall n : nat, Sg n -> n.-tuple Term -> Term". *)
+
+Inductive Term :=
+  | Tvar : nat -> Term
+  | Tope n : Sg n -> Vector.t Term n -> Term.
+(* success *)
